@prefix : <http://data.open.ac.uk/ontology/newsclassification/nco+schema.org#> .
@prefix dul: <http://www.ontologydesignpatterns.org/ont/dul/d0.owl#> .
@prefix nao: <http://purl.org/news/angles/> .
@prefix nco: <http://data.open.ac.uk/ontology/newsclassification/v2#> .
@prefix owl: <http://www.w3.org/2002/07/owl#> .
@prefix rdf: <http://www.w3.org/1999/02/22-rdf-syntax-ns#> .
@prefix xml: <http://www.w3.org/XML/1998/namespace> .
@prefix xsd: <http://www.w3.org/2001/XMLSchema#> .
@prefix iptc: <http://cv.iptc.org/newscodes/mediatopic/> .
@prefix rdfs: <http://www.w3.org/2000/01/rdf-schema#> .
@prefix skos: <http://www.w3.org/2004/02/skos/core#> .
@prefix swrl: <http://www.w3.org/2003/11/swrl#> .
@prefix time: <http://www.w3.org/2006/time#> .
@prefix swrla: <http://swrl.stanford.edu/ontologies/3.3/swrla.owl#> .
@prefix swrlb: <http://www.w3.org/2003/11/swrlb#> .
@prefix terms: <http://purl.org/dc/terms/> .
@prefix schema: <https://schema.org/> .
@prefix nco_schema: <http://data.open.ac.uk/ontology/newsclassification/nco_schema.org#> .
@base <http://data.open.ac.uk/ontology/newsclassification/nco_schema.org#> .

<http://data.open.ac.uk/ontology/newsclassification/nco_schema.org> rdf:type owl:Ontology ;
                                                                     owl:versionIRI <http://github.com/EnricoMotta/ontologies/newsclassification/nco+schema.org/1.0.1> ;
                                                                     owl:imports <http://github.com/EnricoMotta/ontologies/newsclassification/v2.2.0> ;
                                                                     terms:title "News Classification Ontology (NCO)"@en ;
                                                                     rdfs:comment "This ontology integrates the News Classification Ontology (NCO) v2.2 with Schema.Org.  The purpose of this integration is to import the taxonomy of organizations available in Schema.Org into NCO."@en .

#################################################################
#    Annotation properties
#################################################################

###  http://purl.org/dc/terms/title
terms:title rdf:type owl:AnnotationProperty .


#################################################################
#    Classes
#################################################################

###  http://data.open.ac.uk/ontology/newsclassification/v2#Organization
nco:Organization rdf:type owl:Class ;
                 owl:equivalentClass <http://schema.org/Organization> .


###  http://data.open.ac.uk/ontology/newsclassification/v2#PersonOrOganization
nco:PersonOrOganization rdf:type owl:Class .


###  http://schema.org/Organization
<http://schema.org/Organization> rdf:type owl:Class ;
                                 rdfs:subClassOf nco:PersonOrOganization .


#################################################################
#    Annotations
#################################################################

nco:Publisher rdfs:comment "A publisher can be either a person or an organization" .


#################################################################
#    Inverse Object Properties for NCO
#################################################################

### nco:isNewsSourceOf (inverse of nco:hasNewsSource)
nco:isNewsSourceOf rdf:type owl:ObjectProperty ;
    owl:inverseOf nco:hasNewsSource ;
    rdfs:domain nco:NewsSource ;
    rdfs:range nco:NewsItem ;
    rdfs:label "is news source of"@en ;
    rdfs:comment "Inverse property of hasNewsSource. Relates a NewsSource to the NewsItems it is source of."@en .

nco:hasNewsSource owl:inverseOf nco:isNewsSourceOf .

### nco:isPublisherOf (inverse of nco:hasPublisher)
nco:isPublisherOf rdf:type owl:ObjectProperty ;
    owl:inverseOf nco:hasPublisher ;
    rdfs:domain nco:Publisher ;
    rdfs:range nco:NewsSource ;
    rdfs:label "is publisher of"@en ;
    rdfs:comment "Inverse property of hasPublisher. Relates a Publisher to the NewsSources it publishes."@en .

nco:hasPublisher owl:inverseOf nco:isPublisherOf .

### nco:isAgentOf (inverse of nco:hasAgent)
nco:isAgentOf rdf:type owl:ObjectProperty ;
    owl:inverseOf nco:hasAgent ;
    rdfs:domain nco:Agent ;
    rdfs:range nco:AgentComponent ;
    rdfs:label "is agent of"@en ;
    rdfs:comment "Inverse property of hasAgent. Relates an Agent to the AgentComponents it is part of."@en .

nco:hasAgent owl:inverseOf nco:isAgentOf .

### nco:isAgentRoleOf (inverse of nco:hasAgentRole)
nco:isAgentRoleOf rdf:type owl:ObjectProperty ;
    owl:inverseOf nco:hasAgentRole ;
    rdfs:domain nco:AgentRole ;
    rdfs:range nco:AgentComponent ;
    rdfs:label "is agent role of"@en ;
    rdfs:comment "Inverse property of hasAgentRole. Relates an AgentRole to the AgentComponents it is assigned to."@en .

nco:hasAgentRole owl:inverseOf nco:isAgentRoleOf .

### nco:isUtteranceOf (inverse of nco:hasUtterance)
nco:isUtteranceOf rdf:type owl:ObjectProperty ;
    owl:inverseOf nco:hasUtterance ;
    rdfs:domain nco:Utterance ;
    rdfs:range nco:Claim ;
    rdfs:label "is utterance of"@en ;
    rdfs:comment "Inverse property of hasUtterance. Relates an Utterance to the Claim it belongs to."@en .

nco:hasUtterance owl:inverseOf nco:isUtteranceOf .

### nco:isUtteranceTypeOf (inverse of nco:hasUtteranceType)
nco:isUtteranceTypeOf rdf:type owl:ObjectProperty ;
    owl:inverseOf nco:hasUtteranceType ;
    rdfs:domain nco:UtteranceType ;
    rdfs:range nco:Utterance ;
    rdfs:label "is utterance type of"@en ;
    rdfs:comment "Inverse property of hasUtteranceType. Relates an UtteranceType to the Utterances it classifies."@en .

nco:hasUtteranceType owl:inverseOf nco:isUtteranceTypeOf .

###  Generated by the OWL API (version 4.5.29.2024-05-13T12:11:03Z) https://github.com/owlcs/owlapi
